\subsection{Notation}\label{sec:notation}

Let \((i)^{-}\) be the inverse of \((i)\) such that
\(\big((i)\big)^- = i\).
\begin{example}
  \begin{tabular}{cccc}
    \toprule
    \(i\) & \(\beta\) & \((i)\) & \((i)^-\) \\
    \midrule
    1     & 1         & 2       & 3         \\
    2     & -3        & 3       & 1         \\
    3     & 2         & 1       & 2         \\
    \bottomrule
  \end{tabular}
\end{example}
Note that this means that
\[
  J(\beta) = \sum_{j=1}^p \lambda_j |\beta_{(j)}|
           = \sum_{j=1}^p \lambda_{(j)^-}|\beta_j|.
\]
